Cell : cleanup a bit. Transform the various primitices into functions.

theories/typing/unsafe/cell.v
@@ -13,39 +13,65 @@ Section cell.
   Program Definition cell (ty : type) :=
     {| ty_size := ty.(ty_size);
        ty_own := ty.(ty_own);
-       ty_shr κ tid l := (&na{κ, tid, shrN.@l} l ↦∗: ty.(ty_own) tid)%I |}.
+       ty_shr κ tid l :=
+         (∃ P, ▷ □ (P ↔ l ↦∗: ty.(ty_own) tid) ∗ &na{κ, tid, shrN.@l}P)%I |}.
   Next Obligation. apply ty_size_eq. Qed.
   Next Obligation.
-    iIntros (ty E κ l tid q ?) "#LFT Hown $". by iApply bor_na.
+    iIntros (ty E κ l tid q ?) "#LFT Hown $". iExists _.
+    iMod (bor_na with "Hown") as "$". set_solver. iIntros "!>!>!#". iSplit; auto.
   Qed.
   Next Obligation.
-    iIntros (ty ?? tid l) "#LFT". iApply na_bor_shorten.
+    iIntros (ty ?? tid l) "#LFT #H⊑ H". iDestruct "H" as (P) "[??]".
+    iExists _. iFrame. by iApply (na_bor_shorten with "H⊑").
   Qed.
 
-  (* TODO: non-expansiveness, proper wrt. eqtype *)
+  Global Instance cell_ne n : Proper (dist n ==> dist n) cell.
+  Proof.
+    intros ?? EQ. split; [split|]; simpl; try apply EQ.
+    intros κ tid l. repeat (apply EQ || f_contractive || f_equiv).
+  Qed.
+
+  Global Instance cell_mono E L : Proper (eqtype E L ==> subtype E L) cell.
+  Proof.
+    iIntros (?? EQ%eqtype_unfold) "#LFT #HE #HL".
+    iDestruct (EQ with "LFT HE HL") as "(% & #Hown & #Hshr)".
+    iSplit; [done|iSplit; iIntros "!# * H"].
+    - iApply ("Hown" with "H").
+    - iDestruct "H" as (P) "[#HP H]". iExists P. iFrame. iSplit; iNext; iIntros "!# H".
+      + iDestruct ("HP" with "H") as (vl) "[??]". iExists vl. iFrame. by iApply "Hown".
+      + iApply "HP". iDestruct "H" as (vl) "[??]". iExists vl. iFrame. by iApply "Hown".
+  Qed.
+  Lemma cell_mono' E L ty1 ty2 : eqtype E L ty1 ty2 → subtype E L (cell ty1) (cell ty2).
+  Proof. eapply cell_mono. Qed.
+  Global Instance cell_proper E L : Proper (eqtype E L ==> eqtype E L) cell.
+  Proof. by split; apply cell_mono. Qed.
+  Lemma cell_proper' E L ty1 ty2 : eqtype E L ty1 ty2 → eqtype E L (cell ty1) (cell ty2).
+  Proof. eapply cell_proper. Qed.
 
   Global Instance cell_copy :
     Copy ty → Copy (cell ty).
   Proof.
     intros ty Hcopy. split; first by intros; simpl; apply _.
     iIntros (κ tid E F l q ??) "#LFT #Hshr Htl Htok". iExists 1%Qp. simpl in *.
+    iDestruct "Hshr" as (P) "[HP Hshr]".
     (* Size 0 needs a special case as we can't keep the thread-local invariant open. *)
     destruct (ty_size ty) as [|sz] eqn:Hsz.
     { iMod (na_bor_acc with "LFT Hshr Htok Htl") as "(Hown & Htl & Hclose)"; [solve_ndisj..|].
-      iDestruct "Hown" as (vl) "[H↦ #Hown]".
+      iDestruct ("HP" with "Hown") as (vl) "[H↦ #Hown]".
       simpl. assert (F ∖ ∅ = F) as -> by set_solver+.
       iDestruct (ty_size_eq with "Hown") as "#>%". rewrite ->Hsz in *.
       iMod ("Hclose" with "[H↦] Htl") as "[$ $]".
-      { iExists vl. by iFrame. }
+      { iApply "HP". iExists vl. by iFrame. }
       iModIntro. iSplitL "".
       { iNext. iExists vl. destruct vl; last done. iFrame "Hown".
         by iApply heap_mapsto_vec_nil. }
       by iIntros "$ _". }
     (* Now we are in the non-0 case. *)
-    iMod (na_bor_acc with "LFT Hshr Htok Htl") as "($ & Htl & Hclose)"; [solve_ndisj..|].
+    iMod (na_bor_acc with "LFT Hshr Htok Htl") as "(H & Htl & Hclose)"; [solve_ndisj..|].
+    iDestruct ("HP" with "H") as "$".
     iDestruct (na_own_acc with "Htl") as "($ & Hclose')"; first by set_solver.
     iIntros "!> Htl Hown". iPoseProof ("Hclose'" with "Htl") as "Htl".
-    iMod ("Hclose" with "Hown Htl") as "[$ $]". done.
+    iMod ("Hclose" with "[Hown] Htl") as "[$ $]"; last done. by iApply "HP".
   Qed.
 
   Global Instance cell_send :
@@ -56,37 +82,60 @@ End cell.
 Section typing.
   Context `{typeG Σ}.
 
-  (* All of these are of course actual code in Rust, but somehow this is more fun. *)
+  (* Constructing a cell. *)
+  Definition cell_new : val := funrec: <> ["x"] := "return" ["x"].
 
-  (* Constructing a cell is a coercion. *)
-  Lemma tctx_mk_cell E L ty p :
-    tctx_incl E L [p ◁ ty] [p ◁ cell ty].
+  Lemma cell_new_type ty :
+    typed_instruction_ty [] [] [] cell_new
+        (fn (λ _, [])%EL (λ _, [# box ty]) (λ _:(), box (cell ty))).
   Proof.
+    apply type_fn; [apply _..|]. move=>/= _ ret arg. inv_vec arg=>x. simpl_subst.
+    eapply (type_jump [_]); first solve_typing.
     iIntros (???) "#LFT $ $ Hty". rewrite !tctx_interp_singleton /=. done.
   Qed.
 
-  (* Same for the other direction *)
-  Lemma tctx_unmk_cell E L ty p :
-    tctx_incl E L [p ◁ cell ty] [p ◁ ty].
+  (* Same for the other direction.
+     FIXME : this does not exist in Rust.*)
+  Definition cell_into_inner : val := funrec: <> ["x"] := "return" ["x"].
+
+  Lemma cell_into_inner_type ty :
+    typed_instruction_ty [] [] [] cell_into_inner
+        (fn (λ _, [])%EL (λ _, [# box (cell ty)]) (λ _:(), box ty)).
   Proof.
+    apply type_fn; [apply _..|]. move=>/= _ ret arg. inv_vec arg=>x. simpl_subst.
+    eapply (type_jump [_]); first solve_typing.
     iIntros (???) "#LFT $ $ Hty". rewrite !tctx_interp_singleton /=. done.
   Qed.
 
-  Lemma read_cell E L κ ty :
-    Copy ty → lctx_lft_alive E L κ →
-    typed_read E L (&shr{κ} cell ty) ty (&shr{κ} cell ty).
-  Proof. intros ??. exact: read_shr. Qed.
+  (* Reading from a cell *)
+  Definition cell_get ty : val :=
+    funrec: <> ["x"] :=
+      let: "x'" := !"x" in
+      letalloc: "r" <-{ty.(ty_size)} !"x'" in
+      delete [ #1; "x"];; "return" ["r"].
 
-  (* Writing actually needs code; typed_write can't have thread tokens. *)
-  Definition cell_write ty : val :=
+  Lemma cell_get_type `(!Copy ty) :
+    typed_instruction_ty [] [] [] (cell_get ty)
+        (fn (λ α, [☀α])%EL (λ α, [# box (&shr{α} (cell ty))])%T (λ _, box ty)).
+  Proof.
+    apply type_fn; [apply _..|]. move=>/= α ret arg. inv_vec arg=>x. simpl_subst.
+    eapply type_deref; [solve_typing..|apply read_own_move|done|]=>x'. simpl_subst.
+    eapply type_letalloc_n; [solve_typing..| |solve_typing|intros r; simpl_subst].
+    { apply (read_shr _ _ _ (cell ty)); solve_typing. }
+    eapply type_delete; [solve_typing..|].
+    eapply (type_jump [_]); solve_typing.
+  Qed.
+
+  (* Writing to a cell *)
+  Definition cell_set ty : val :=
     funrec: <> ["c"; "x"] :=
        let: "c'" := !"c" in
        "c'" <-{ty.(ty_size)} !"x";;
        let: "r" := new [ #0 ] in
        delete [ #1; "c"] ;; delete [ #ty.(ty_size); "x"] ;; "return" ["r"].
 
-  Lemma cell_write_type ty :
-    typed_instruction_ty [] [] [] (cell_write ty)
+  Lemma cell_set_type ty :
+    typed_instruction_ty [] [] [] (cell_set ty)
         (fn (λ α, [☀α])%EL (λ α, [# box (&shr{α} cell ty); box ty])
             (λ α, box unit)).
   Proof.
@@ -101,19 +150,20 @@ Section typing.
       rewrite tctx_interp_cons tctx_interp_singleton !tctx_hasty_val.
       iIntros "[Hc' Hx]". rewrite {1}/elctx_interp big_opL_singleton /=.
       iDestruct "Hc'" as (l) "[EQ #Hshr]". iDestruct "EQ" as %[=->].
+      iDestruct "Hshr" as (P) "[#HP #Hshr]".
       iDestruct "Hx" as (l') "[EQ [Hown >H†]]". iDestruct "EQ" as %[=->].
       iDestruct "Hown" as (vl') "[>H↦' Hown']".
       iMod (na_bor_acc with "LFT Hshr HE Htl") as "(Hown & Htl & Hclose)"; [solve_ndisj..|].
-      iDestruct "Hown" as (vl) "[>H↦ Hown]".
+      iDestruct ("HP" with "Hown") as (vl) "[>H↦ Hown]".
       iDestruct (ty_size_eq with "Hown") as "#>%".
       iDestruct (ty_size_eq with "Hown'") as "#>%".
       iApply wp_fupd. iApply (wp_memcpy with "[$HEAP $H↦ $H↦']"); [done..|].
       iNext. iIntros "[H↦ H↦']". rewrite {1}/elctx_interp big_opL_singleton /=.
       iMod ("Hclose" with "[H↦ Hown'] Htl") as "[$ $]".
-      { iExists vl'. by iFrame. }
+      { iApply "HP". iExists vl'. by iFrame. }
       rewrite tctx_interp_cons tctx_interp_singleton !tctx_hasty_val' //.
       iSplitR; iModIntro.
-      - iExists _. iSplit; done.
+      - iExists _. simpl. eauto.
       - iExists _. iSplit; first done. iFrame. iExists _. iFrame.
         rewrite uninit_own. auto. }
     intros v. simpl_subst. clear v.
@@ -124,5 +174,20 @@ Section typing.
     eapply (type_jump [_]); solve_typing.
   Qed.
 
-  (* TODO: get_mut *)
+  (* Reading from a cell *)
+  Definition cell_get_mut : val :=
+    funrec: <> ["x"] := "return" ["x"].
+
+  Lemma cell_get_mut_type `(!Copy ty) :
+    typed_instruction_ty [] [] [] cell_get_mut
+      (fn (λ α, [☀α])%EL (λ α, [# box (&uniq{α} (cell ty))])%T
+          (λ α, box (&uniq{α} ty))%T).
+  Proof.
+    apply type_fn; [apply _..|]. move=>/= α ret arg. inv_vec arg=>x. simpl_subst.
+    eapply (type_jump [_]). solve_typing. rewrite /tctx_incl /=.
+    iIntros (???) "_ $$". rewrite !tctx_interp_singleton /tctx_elt_interp /=.
+    by iIntros "$".
+  Qed.
 End typing.
+
+Hint Resolve cell_mono' cell_proper' : lrust_typing.
